% 导言区
\documentclass{article}
\usepackage{ctex}
\usepackage {amsmath}

% 正文区
\begin{document}
	
	\[
		\alpha^3 + \beta^2 + \gamma = 0
	\]
	
	$\sin^2 + \cos^2 = 1$
	
	$y = \log_2 x + \ln x + \sqrt{x^2+y^2}$

	
	\begin{equation}
		J(A,B) = \frac{|A \bigcap B|}{|A \bigcup B|} \label{eq}
	\end{equation}
	
	\begin{equation}
		a+b=\sqrt{\frac{a}{b}}\label{eq}
	\end{equation}
	
	交换律见公式\ref{eq:commutative}
	\begin{equation}
		a+b=b+a \label{eq:commutative}
	\end{equation}
	
	\begin{equation}
		\begin{aligned}
		Similarity &= \cos \theta\\
		&= \frac{A·B}{||A|| ||B||}\\
		&= \frac{\sum_{i=1}^{n}A_i \times B_i}{\sqrt{\sum_{i=1}^{n}A_i^2} \times \sqrt{\sum_{i=1}^{n}B_i^2}}
		\end{aligned}
		\label{eq}
	\end{equation}
	
	
	\[
	\begin{matrix}
		a & b & c \\
		d & e & f \\
		g & h & i
	\end{matrix} \qquad
	% 小括号
	\begin{pmatrix}
	a & b & c \\
	d & e & f \\
	g & h & i
	\end{pmatrix} \qquad
	% 中括号
	\begin{bmatrix}
	a & b & c \\
	d & e & f \\
	g & h & i
	\end{bmatrix} \qquad
	% 大括号
	\begin{Bmatrix}
	a & b & c \\
	d & e & f \\
	g & h & i
	\end{Bmatrix}  \qquad
	% 单竖线
	\begin{vmatrix}
	a & b & c \\
	d & e & f \\
	g & h & i
	\end{vmatrix}  \qquad
	% 双竖线
	\begin{Vmatrix}
	a & b & c \\
	d & e & f \\
	g & h & i
	\end{Vmatrix}  \qquad
	\]
	
	$$
	A_{m,n} = 
	\begin{pmatrix}
		a_{1,1} & a_{1,2} & \cdots & a_{1,n} \\
		a_{2,1} & a_{2,2} & \cdots & a_{2,n} \\
		\vdots  & \vdots  & \ddots & \vdots  \\
		a_{m,1} & a_{m,2} & \cdots & a_{m,n} 
	\end{pmatrix}
	$$
	
	$$
	M = \begin{bmatrix}
		\frac{5}{6} & \frac{1}{6} & 0           \\[0.3em]
		\frac{5}{6} & 0           & \frac{1}{6} \\[0.3em]
		0           & \frac{5}{6} & \frac{1}{6}
	\end{bmatrix}
	$$
	
	$$
	M = \bordermatrix{~ & x & y \cr
		A & 1 & 0 \cr
		B & 0 & 1 \cr}
	$$

	$$
	A = \begin{bmatrix}
	a_{11} & \dots & a_{1n} \\
	& \ddots & \vdots \\
	0 & & a_{nn}
	\end{bmatrix}_{n \times n}
	$$
	
	$$
	f(n) =
	\begin{cases}
	n/2,  & \text{if $n$ is even} \\
	3n+1, & \text{if $n$ is odd}
	\end{cases}
	$$
	
	
	$$
	\left\{ 
	\begin{array}{c}
	a_1x+b_1y+c_1z=d_1 \\ 
	a_2x+b_2y+c_2z=d_2 \\ 
	a_3x+b_3y+c_3z=d_3
	\end{array}
	\right. 
	$$
	
	$$
	\frac{\partial J(\theta)}{\partial\theta_j}=-\frac1m\sum_{i=0}^m(y^i-h_\theta(x^i))x^i_j
	$$
	
	\begin{gather}
	a + b = b + a \\
	a + b + c = 0 \\
	a^2 + b^2 = 1
	\end{gather}
	
		
\end{document}